Add new types and helper functions for withdrawal and execution

src/dafny/beacon/Helpers.dfy
@@ -200,8 +200,53 @@ module BeaconHelpers {
         forall i,j :: 0 <= i < j < |indices| ==> indices[i] < indices[j]
     }
 
-    
-    ///////////////////////////////////////////////////////////////////////////////////////////
+    /**
+     * Check if ``validator`` has an 0x01 prefixed "eth1" withdrawal credential.
+     *
+     * @param  validator                A validator.
+     * @return                          True if the validator has an 0x01 prefixed "eth1"
+     */
+    // Define a method to check if a validator has an 0x01 prefixed "eth1" withdrawal credential
+    predicate method has_eth1_withdrawal_credential(validator: Validator)
+    {
+        // Check if the first byte of withdrawal_credentials is equal to the ETH1_ADDRESS_WITHDRAWAL_PREFIX
+        (validator.withdrawal_credentials[0] == ETH1_ADDRESS_WITHDRAWAL_PREFIX)
+    }
+
+    /**
+     * Check if ``validator`` is fully withdrawable.
+     *
+     * @param validator                A validator.
+     * @param balance                  A Gwei amount.
+     * @param epoch                    An epoch.
+     * @return                         True if the validator is fully withdrawable.
+     */
+    predicate method is_fully_withdrawable_validator(validator: Validator, balance: Gwei, epoch: Epoch)
+    {   
+        has_eth1_withdrawal_credential &&
+         validator.withdrawable_epoch <= epoch &&
+          balance > 0
+    }
+
+    /**
+     * Check if ``validator`` is partially withdrawable.
+     *
+     * @param validator                A validator.
+     * @param balance                  A Gwei amount.
+     * @param epoch                    An epoch.
+     *
+     * @return                         True if the validator is partially withdrawable.
+     */
+    predicate method is_partially_withdrawable_validator(validator: Validator, balance: Gwei, epoch: Epoch)
+    {
+        has_eth1_withdrawal_credential(validator) &&
+         validator.effective_balance == MAX_EFFECTIVE_BALANCE &&
+          balance > MAX_EFFECTIVE_BALANCE
+    }
+
+
+    ///////////////////////////////
+    ////////////////////////////////////////////////////////////
     //  Helper functions - Misc 
     //  @note   compute_fork_data_root, compute_fork_digest, compute_domain and
     //          compute_signing_root are not required to implement this model.
